define basic terms from complexity theory (up to DTIME)
use definitions from AFP entry "Universal_Turing_Machine"

papers/116_stefan_rass/complexity.thy
@@ -1,20 +1,119 @@
 theory complexity
-  imports Main "HOL-Library.BigO"
+  imports Main gn "Universal_Turing_Machine.UTM"
 begin
 
-(*a locale to capture our intuition of Turing machines*)
-locale TM =
-  fixes \<Gamma>\<^sub>i\<^sub>n :: "'a set" (*input alphabet*)
-  fixes k :: nat (*tape count*)
-  fixes time :: "'a list \<Rightarrow> nat"
-  fixes space :: "'a list \<Rightarrow> nat"
+subsection\<open>Termination\<close>
 
-  assumes input_alphabet_finite: "finite \<Gamma>\<^sub>i\<^sub>n"
+text\<open>The tape size can not use the universal function \<^term>\<open>size\<close>, since for any pair \<^term>\<open>p = (a, b)\<close>, \<^term>\<open>size p = 1\<close>.\<close>
+fun tape_size :: "tape \<Rightarrow> nat" \<comment> \<open>using \<open>fun\<close> since \<open>definition\<close> does not recognize patterns like \<^term>\<open>(l, r)\<close>\<close>
+  where "tape_size (l, r) = length l + length r"
 
-  (*in one step only k cells can be visited*)
-  assumes "space x \<le> k * time x"
-begin
- 
-end
+text\<open>The time restriction predicate is similar to \<^term>\<open>Hoare_halt\<close>, but includes a maximum number of steps.\<close>
+definition time_restricted :: "(nat \<Rightarrow> nat) \<Rightarrow> tprog0 \<Rightarrow> bool"
+  where "time_restricted T p \<equiv> \<forall>tp. \<exists>n.
+            n \<le> T (tape_size tp)
+          \<and> is_final (steps0 (1, tp) p n)"
+
+(* TODO (?) notation: \<open>p terminates_in_time T\<close> *)
+
+text\<open>\<open>time\<^sub>M(x)\<close> is the number of steps until the computation of \<open>M\<close> halts on input \<open>x\<close>\<close>
+definition time :: "tprog0 \<Rightarrow> tape \<Rightarrow> nat option"
+  where "time p tp = 
+    (if \<exists>n. is_final (steps0 (1, tp) p n) then Some (LEAST n. is_final (steps0 (1, tp) p n)) else None)"
+
+lemma "time_restricted T p \<longleftrightarrow> (\<forall>tp. the (time p tp) \<le> T (tape_size tp))"
+proof (intro iffI allI)
+  fix tp
+  assume "time_restricted T p"
+  then have e: "\<exists>n. n \<le> T (tape_size tp) \<and> is_final (steps0 (1, tp) p n)" unfolding time_restricted_def ..
+  then obtain n where "n \<le> T (tape_size tp)" and nH: "is_final (steps0 (1, tp) p n)" by blast
+
+  have "the (time p tp) = (LEAST n. is_final (steps0 (1, tp) p n))" unfolding time_def using e by auto
+  also have "... \<le> n" using Least_le nH .
+  also note \<open>n \<le> T (tape_size tp)\<close>
+  finally show "the (time p tp) \<le> T (tape_size tp)" .
+next
+  assume "\<forall>tp. the (time p tp) \<le> T (tape_size tp)"
+  then show "time_restricted T p" unfolding time_def time_restricted_def sorry
+  oops
+
+
+subsection\<open>Encoding\<close>
+
+text\<open>Encoding binary words as TM tape cells: \<^term>\<open>Num.Bit1\<close> is encoded as \<^term>\<open>[Oc, Oc]\<close> and \<^term>\<open>Num.Bit1\<close> as term>\<open>[Oc, Bk]\<close>.
+  Thus, the ends of an encoded term can be marked with the pattern \<^term>\<open>[Bk, Bk]\<close>.\<close>
+fun encode_word :: "word \<Rightarrow> cell list"
+  where "encode_word Num.One = []"
+      | "encode_word (Num.Bit0 w) = Oc # Bk # encode_word w"
+      | "encode_word (Num.Bit1 w) = Oc # Oc # encode_word w"
+
+fun is_encoded_word :: "cell list \<Rightarrow> bool"
+  where "is_encoded_word [] = True"
+      | "is_encoded_word (Oc # _ # cs) = is_encoded_word cs"
+      | "is_encoded_word _ = False"
+
+fun decode_word :: "cell list \<Rightarrow> word"
+  where "decode_word (Oc # Bk # cs) = Num.Bit0 (decode_word cs)"
+      | "decode_word (Oc # Oc # cs) = Num.Bit1 (decode_word cs)"
+      | "decode_word _ = Num.One"
+
+
+lemma encode_decode_word: "decode_word (encode_word w) = w" 
+  by (induction w) simp_all
+
+lemma decode_encode_word:
+  "is_encoded_word cs \<Longrightarrow> encode_word (decode_word cs) = cs" 
+  (is "?ie cs \<Longrightarrow> ?de cs = cs")
+proof (induction cs rule: is_encoded_word.induct)
+  case (2 c cs) (* cs = Oc # c # cs *)
+  from \<open>?ie (Oc # c # cs)\<close> have "?ie cs" by simp
+  with "2.IH" have IH: "?de cs = cs" .
+  then show ?case by (cases c) simp_all
+qed (* cases "cs = []", "cs = Bk # _", "cs = [_]" by *) simp_all
+
+
+subsection\<open>Deciding Languages\<close>
+
+\<comment> \<open>TODO \<^term>\<open>L\<close> is recognized as the constant of type \<^typ>\<open>action\<close> ("move head left").
+    Since \<open>L\<close> is a typical name for unspecified languages in the literature, 
+    being unable to use it as variable name is annoying.\<close>
+
+text\<open>A TM \<^term>\<open>p\<close> is considered to decide a language \<^term>\<open>l\<close>, iff for every possible word \<^term>\<open>w\<close>
+  it correctly calculates language membership. 
+  That is, for \<^term>\<open>w \<in> l\<close> the computation results in \<^term>\<open>Oc\<close> under the TM head, 
+  and for \<^term>\<open>w \<notin> l\<close> in \<^term>\<open>Bk\<close>.
+  The head is over the first cell of the right tape. 
+  That is for \<^term>\<open>tp = (l, x # r)\<close>, the symbol under the head is \<open>x\<close>, or \<open>hd (snd tp)\<close>\<close>
+definition decides :: "lang \<Rightarrow> tprog0 \<Rightarrow> bool" 
+  where "decides l p \<equiv> \<forall>w. Hoare_halt
+    (\<lambda>tp. tp = ([], encode_word w)) p (\<lambda>tp. hd (snd tp) = (if w \<in> l then Oc else Bk))"
+
+(* TODO (?) notation: \<open>l decides p\<close> *)
+
+
+subsection\<open>DTIME\<close>
+
+text\<open>\<open>DTIME(T)\<close> is the set of languages decided by TMs in time \<open>T\<close> or less.\<close>
+definition DTIME :: "(nat \<Rightarrow> nat) \<Rightarrow> lang set"
+  where "DTIME T \<equiv> {l. \<exists>p. decides l p \<and> time_restricted T p}"
+
+lemma in_dtimeI[intro]:
+  assumes "decides l p"
+    and "time_restricted T p"
+  shows "l \<in> DTIME T"
+  unfolding DTIME_def using assms by blast
+
+lemma in_dtimeE[elim]:
+  assumes "l \<in> DTIME T"
+  obtains p
+  where "decides l p" 
+    and "time_restricted T p"
+  using assms unfolding DTIME_def by blast
+
+lemma in_dtimeE'[elim]:
+  assumes "l \<in> DTIME T"
+  shows "\<exists>p. decides l p \<and> time_restricted T p"
+  using assms unfolding DTIME_def ..
+
 
 end
